Fix typo 256 -> 128

frodo/code/Hacl.Impl.Frodo.Gen.fst
@@ -37,13 +37,13 @@ val gen_inv:
   -> Type0
 let gen_inv h0 h1 h2 n seed_len seed r res i j =
   B.live h2 res /\ B.live h2 seed /\ B.live h2 r /\
-  disjoint seed res /\ disjoint r res /\
-  modifies (loc_buffer res) h1 h2 /\ j <= v n /\
+  modifies (loc_buffer res) h1 h2 /\ 
+  j <= v n /\
   (forall (i0:size_nat{i0 < v i}) (j:size_nat{j < v n}). get h2 res i0 j == get h1 res i0 j) /\
   (forall (j0:size_nat{j0 < j}). get h2 res (v i) j0 == S.frodo_gen_matrix_cshake_fc (v n) (v seed_len) (as_seq h0 seed) (v i) j0) /\
   (forall (j0:size_nat{j <= j0 /\ j0 < v n}). get h2 res (v i) j0 == get h0 res (v i) j0) /\
   (forall (i0:size_nat{v i < i0 /\ i0 < v n}) (j:size_nat{j < v n}). get h2 res i0 j == get h0 res i0 j) /\
-  as_seq h1 r == Spec.Frodo.Keccak.cshake256_frodo (v seed_len) (as_seq h0 seed) (u16 (256 + v i)) (2 * v n) /\
+  as_seq h1 r == Spec.Frodo.Keccak.cshake128_frodo (v seed_len) (as_seq h0 seed) (u16 (256 + v i)) (2 * v n) /\
   as_seq h1 r == as_seq h2 r
 
 inline_for_extraction noextract private
@@ -54,15 +54,15 @@ val frodo_gen_matrix_cshake_fc:
   -> seed_len:size_t{v seed_len > 0}
   -> seed:lbytes seed_len
   -> r:lbytes (size 2 *! n)
-  -> res0:matrix_t n n
+  -> res:matrix_t n n{disjoint seed res /\ disjoint r res}
   -> i:size_t{v i < v n}
   -> j:size_t{v j < v n}
   -> Stack unit
-    (requires fun h2 -> gen_inv h0 h1 h2 n seed_len seed r res0 i (v j))
-    (ensures  fun _ _ h2 -> gen_inv h0 h1 h2 n seed_len seed r res0 i (v j + 1))
-let frodo_gen_matrix_cshake_fc h0 h1 n seed_len seed r res0 i j =
+    (requires fun h2 -> gen_inv h0 h1 h2 n seed_len seed r res i (v j))
+    (ensures  fun _ _ h2 -> gen_inv h0 h1 h2 n seed_len seed r res i (v j + 1))
+let frodo_gen_matrix_cshake_fc h0 h1 n seed_len seed r res i j =
   let resij = sub r (size 2 *! j) (size 2) in
-  mset res0 i j (uint_from_bytes_le resij)
+  mset res i j (uint_from_bytes_le resij)
 
 private
 val gen_inner_inv:
@@ -72,12 +72,11 @@ val gen_inner_inv:
   -> seed_len:size_t{v seed_len > 0}
   -> seed:lbytes seed_len
   -> res:matrix_t n n
-  -> r:lbytes (size 2 *! n)
+  -> r:lbytes (size 2 *! n){disjoint seed res /\ disjoint seed r /\ disjoint r res}
   -> i:size_nat{i <= v n}
   -> Type0
 let gen_inner_inv h0 h1 n seed_len seed res r i =
   B.live h1 r /\ B.live h1 res /\ B.live h1 seed /\
-  disjoint seed res /\ disjoint seed r /\ disjoint r res /\
   modifies (loc_union (loc_buffer res) (loc_buffer r)) h0 h1 /\ as_seq h0 seed == as_seq h1 seed /\
   (forall (i0:size_nat{i0 < i}) (j:size_nat{j < v n}). get h1 res i0 j == S.frodo_gen_matrix_cshake_fc (v n) (v seed_len) (as_seq h0 seed) i0 j) /\
   (forall (i0:size_nat{i <= i0 /\ i0 < v n}) (j:size_nat{j < v n}). get h1 res i0 j == get h0 res i0 j)
@@ -92,19 +91,19 @@ val frodo_gen_matrix_cshake_inner:
   -> r:lbytes (size 2 *! n)
   -> i:size_t{v i < v n}
   -> Stack unit
-    (requires fun h1 -> gen_inner_inv h0 h1 n seed_len seed res r (v i))
+    (requires fun h1 -> 
+      disjoint seed res /\ disjoint seed r /\ disjoint r res /\
+      gen_inner_inv h0 h1 n seed_len seed res r (v i))
     (ensures  fun _ _ h1 -> gen_inner_inv h0 h1 n seed_len seed res r (v i + 1))
 let frodo_gen_matrix_cshake_inner h0 n seed_len seed res r i =
   let h0 = ST.get () in
   let ctr = size_to_uint32 (size 256 +. i) in
   uintv_extensionality (to_u16 (size_to_uint32 (size 256 +. i))) (u16 (256 + v i));
-  cshake128_frodo seed_len seed (to_u16 ctr) (size 2 *! n) r;
+  Hacl.Keccak.cshake128_frodo seed_len seed (to_u16 ctr) (size 2 *! n) r;
   let h1 = ST.get () in
   Lib.Loops.for (size 0) n
     (fun h2 j -> gen_inv h0 h1 h2 n seed_len seed r res i j)
-    (fun j -> frodo_gen_matrix_cshake_fc h0 h1 n seed_len seed r res i j);
-  let h2 = ST.get () in
-  assert (gen_inner_inv h0 h2 n seed_len seed res r (v i + 1))
+    (fun j -> frodo_gen_matrix_cshake_fc h0 h1 n seed_len seed r res i j)
 
 val frodo_gen_matrix_cshake:
     n:size_t{0 < v n /\ 2 * v n < max_size_t /\ 256 + v n < maxint U16 /\ v n * v n < max_size_t}
